Usa ghost variables

Stack.dfy
@@ -1,10 +1,16 @@
 class Stack {
   var arr : array<int>;
   var index : nat;
+  ghost var repr: set<object>;
   ghost var elements: seq<int>;
-  predicate Valid() reads this
+
+  predicate Valid() 
+    reads this, repr
   {
-    0 <= index < arr.Length
+    arr in repr 
+    && arr.Length > 0 
+    && 0 <= index < arr.Length 
+    && elements == arr[0..index]
   }
 
   predicate Empty() reads this
@@ -13,25 +19,21 @@ class Stack {
   }
   predicate Full() reads this
   {
-    index == arr.Length
+    index >= arr.Length
   }
 
   constructor(size: nat) 
     requires size > 0 
     ensures Valid()
     ensures Empty()
+    ensures elements == []
     ensures fresh(arr)
     ensures arr.Length == size
   {
     arr := new int[size];
     elements := [];
     index := 0;
-  }
-
-  method IsEmpty() returns (result : bool)
-    requires Empty()
-  {
-      return true;
+    repr := { arr };
   }
 
   method Top()
@@ -44,18 +46,38 @@ class Stack {
     element := arr[index];
   }
 
-  method Push(element : int) 
-    modifies arr, `index
+  method Elements()
+    returns (element: int)
+    requires !Empty()
     requires Valid()
-    requires !Full()
-    ensures index == old(index) + 1
   {
+    return index;
+  }
+
+  method Push(element : int) 
+    returns (result: bool)
+    modifies arr, `index
+    //requires Valid()
+    //requires !Full()
+   // ensures index == old(index) + 1
+  {
+    if(0 <= index < arr.Length)
+    {
       arr[index] := element;
       index := index+1;
+      return true;
+    }
+    return false;
   }
 
   method Pop() returns (elem : int)
+    modifies this
+    requires Valid()
+    requires !Empty()
+    decreases index
   {
+    elem := arr[index];
+    index := index - 1;
   }
 }
 
@@ -63,10 +85,14 @@ class Stack {
 method Main()
 {
   var stack := new Stack(4);
-  stack.Push(1);
-  stack.Push(2);
-  stack.Push(3);
-  stack.Push(3);
+  var a := stack.Push(1);
+
+ // a := stack.IsFull();
+  a := stack.Push(2);
+  a := stack.Push(3);
+  a := stack.Push(3);
+  a := stack.Push(3);
+  a := stack.Push(3);
 
   //result := stack.Push(5);
   //result := stack.Push(5);
